Draft `delete_unmatchable`

src/deletion.lean
@@ -1,30 +1,22 @@
-
 -- deletion tactics for G&G prover
 
-import meta.expr
-import table
 import robot
 open tactic expr
-open table robot
-universes u v w
-def list.mchoose {m : Type u → Type v} [monad m] {α : Type w} {β : Type u} (f : α → m (option β)) : list α → m (list β)
-| []       := return []
-| (h :: t) := pure (λ (h : option β) (t : list β), option.rec_on h t (λ h, h :: t)) <*> f h <*> list.mchoose t
+open table
 
+namespace robot
 
-
-meta def get_local_consts (e : expr) : table expr := table.from_list $ expr.list_local_const $ e
-
-/- We say that a statement is __dangling__ when it references a variable that no other statements reference. -/
-
-/--Arguments:
+/--
+   We say that a statement is __dangling__ when it references a variable that no other statements reference.  
+   Arguments:
    - an accumulating table of local constants that all of the hyps considered so far.
      add the references of all of the goals to this.
    - an accumulator full of the statements that are dangling
    - a queue of statements yet to check.
+   
    Returns: a list of dangling statements.
 -/
-meta def find_dangling : table expr → list hyp → list hyp → list hyp
+meta def find_dangling : table expr → list statement → list statement → list statement
 | d acc [] := acc
 | d acc  (h :: hs) :=
     find_dangling (d ∪ h.refs) (  
@@ -33,23 +25,86 @@ meta def find_dangling : table expr → list hyp → list hyp → list hyp
         then h :: acc else acc
     ) (hs)
 
-meta def delete_dangling : robot unit :=
-do
-    hyps ← get_hyps,
-    targets ← get_targets,
-    target_deps ← return $ dict.fold (λ _, union) empty $ dict.map (statement.refs) targets,
-    list.mmap' (λ h : statement, clear h.body) $ find_dangling target_deps [] hyps
+meta def delete_dangling : robot unit := do
+    hyps ← robot.get_vuln_hyps,
+    targets ← robot.get_targets,
+    target_deps ← return $ list.foldl union empty $ list.map (statement.refs) targets,
+    list.mmap' (λ h : statement, clear_hyp h.body) $ find_dangling target_deps [] hyps
 
-meta def scratch_tac : tactic unit :=
-do v ← mk_meta_var `(ℕ),
-   e ← mk_app ``eq [v, v],
-   assert_core "h" e,
-   skip
 
-variables a b c : Prop
-example : a → (a → b) → c → b :=
-begin
-  intros h1 h2 h3,
-  scratch_tac,
-  sorry
-end
+/- How to implement 'delete unmatchable'?
+
+    We first need to write a `match` routine.
+    This takes a pi-type hypothesis and attempts to find an argument within 
+
+   Take a hyp H, get its type. We are interested if it is an atomic formula.
+   Now we look at all of the other hypotheses and targets
+   if H can't be applied to any of these then we discard it.
+-/
+
+meta def try_on_all_goals_aux (check : robot unit) : ℕ → robot unit
+|0 := pure ()
+|(nat.succ n) := hypothetically check <|> (rotate 1 *> try_on_all_goals_aux n)
+meta def try_on_all_goals (check : robot unit) : robot unit := num_goals >>= try_on_all_goals_aux check
+
+/--Returns tt if A can be applied as one of the arguments to `H`-/
+meta def is_matchable (A : expr) (H : expr) : robot bool := hypothetically $ 
+    (do
+        m ← mk_mvar,
+        set_goals [m],
+        ms ← apply H {unify := tt, new_goals := new_goals.non_dep_only},
+        cannot_substitute ← get_cannot_substitute H,
+        ms' ← pure $ @list.mapi (name × expr) (expr × table expr) (λ n ⟨l,e⟩, ⟨e, dict.get_default empty n cannot_substitute⟩) ms,
+        -- rotate through all of the goals, seeing if H can be applied.
+        try_on_all_goals (do
+            apply A,
+            @list.mmap' _ _ (expr × table expr) unit (λ ⟨e, x⟩, do 
+                e' ← instantiate_mvars e,
+                assert $ not $ contains e' x,
+                return ()
+            ) ms',
+            return ()
+        ),
+        pure tt)
+    <|> pure ff
+    
+meta def is_atom (h : statement) : robot bool := expr.is_pi <$>  whnf (h.type)
+meta def is_result (h : statement) : robot bool := (bnot ∘ expr.is_pi) <$> whnf (h.type)
+
+meta def delete_unmatchable : robot unit := do
+    lc ← get_hyps, -- [NOTE] needlessly recalculating `refs`
+    atoms ← list.filterm is_atom lc,
+    results ← list.filterm is_result lc,
+    clear_these ← list.filterm (λ a, list.allm (λ r, bnot <$> is_matchable (statement.body a) (statement.body r)) results) atoms,
+    list.mmap' (λ c, clear_hyp (statement.body c)) clear_these
+    
+
+
+
+
+
+
+
+
+end robot
+
+section SCRATCH
+    universe u
+    meta def myfun {α : Type} : α → α → α := λ x _,x 
+    set_option trace.app_builder true
+    meta def mytac : tactic unit := do
+        e ← to_expr $ ```(myfun),
+        fi ← get_fun_info e,
+        trace fi,
+        ssi ← get_subsingleton_info e,
+        trace ssi,
+
+        e2 ← mk_app `myfun [ `(unit.star), `(unit.star)],
+        trace e2
+
+    lemma scratch : true := begin
+        mytac,
+        trivial,
+        sorry,
+    end
+end SCRATCH
